A bit more WIP
this is what i do when i switch between the desktop and laptop.
"use a branch" i will never do such a thing, you heathen!

verify/Enumerate.v
@@ -1,20 +1,65 @@
 (** * Enumerate: TNF enumeration *)
 
+From Coq Require Import List. Import ListNotations.
 From BusyCoq Require Export Permute.
 Set Default Goal Selector "!".
 
 Module Enumerate (Ctx : Ctx).
   Module Permute := Permute Ctx. Export Permute.
 
-Inductive ReachesNZ (tm : TM) : Q -> nat -> Prop :=
-  | Reaches_halt q :
+(** To justify only enumerating machines that start with 1RB, we need
+    to prove that all the other machines won't take many steps to write
+    their first 1 (or a non-zero symbol in the case of non-binary Turing
+    machines). *)
+
+(** [tm] visits the sequence of states [q :: qs] before writing its first
+    non-zero symbol. *)
+Inductive zvisits (tm : TM) : Q -> list Q -> Prop :=
+  | zvisits_halt q :
     tm (q, s0) = None ->
-    ReachesNZ tm q 0
-  | Reaches_now q s d q' :
+    zvisits tm q []
+  | zvisits_nz q s d q' :
     tm (q, s0) = Some (s, d, q') ->
     s <> s0 ->
-    ReachesNZ tm q 0
-  | Reaches_later q d q' n :
+    zvisits tm q []
+  | zvisits_step q d q' qs :
     tm (q, s0) = Some (s0, d, q') ->
-    ReachesNZ tm q' n ->
-    ReachesNZ tm q (S n).
+    zvisits tm q' qs ->
+    zvisits tm q (q' :: qs).
+
+(** This sequence is unique. *)
+
+Lemma zvisits_unique : forall tm qs qs' q,
+  zvisits tm q qs ->
+  zvisits tm q qs' ->
+  qs = qs'.
+Proof.
+  induction qs as [| a qs IH]; introv H1 H2;
+    inverts H1; inverts H2; try congruence.
+  assert (a = q'). { congruence. }
+  subst. f_equal. eauto.
+Qed.
+
+(** Therefore, [q] cannot occur in [qs]. *)
+Lemma zvisits_In_skip : forall tm qs q q',
+  zvisits tm q qs ->
+  In q' qs ->
+  exists qs', zvisits tm q' qs' /\ qs <> qs'.
+Proof.
+  induction qs as [| a qs IH].
+  - contradiction.
+  - introv Hvisits Hin. inverts Hvisits as Etm Hvisits.
+    destruct Hin as [E | Hin]; subst; eauto.
+Qed.
+
+Lemma zvisits_In : forall tm qs q,
+  zvisits tm q qs ->
+  ~ In q qs.
+Proof.
+  introv H1 Hin.
+  apply 
+  induction qs as [| a qs IH].
+  - contradiction.
+  - inverts H1 as Etm H1.
+    * subst a.
+  assert (H2: zvisits tm 
