verify/Pigeonhole.v
@@ -1,0 +1,74 @@
+From Coq Require Import List. Import ListNotations.
+From Coq Require Import Lia.
+From BusyCoq Require Export LibTactics.
+Set Default Goal Selector "!".
+
+(** [repeats xs] if [xs] repeats an element. *)
+Inductive repeats {X : Type} : list X -> Prop :=
+  | repeats_head x xs : In x xs -> repeats (x :: xs)
+  | repeats_cons x xs : repeats xs -> repeats (x :: xs).
+
+Hint Constructors repeats : core.
+
+Lemma in_split : forall (X : Type) (x : X) (l : list X),
+  In x l ->
+  exists l1 l2, l = l1 ++ x :: l2.
+Proof.
+  introv H. induction l as [| a l IH].
+  - inverts H.
+  - destruct H.
+    + subst a. exists (@nil X), l. reflexivity.
+    + specialize (IH H). destruct IH as [l1' [l2' IH]].
+      subst l. exists (a :: l1'), l2'. reflexivity.
+Qed.
+
+Hint Extern 1 (In _ (_ :: _)) => left : core.
+Hint Extern 1 (In _ (_ :: _)) => right : core.
+
+(* See below for the motivation on this lemma. *)
+Lemma insplit_decide : forall (X : Type) (x : X) (l1 l2a l2b : list X),
+  Forall (fun y => In y (l2a ++ x :: l2b)) l1 ->
+  In x l1 \/ Forall (fun y => In y (l2a ++ l2b)) l1.
+Proof.
+  introv Hsubset.
+  induction l1 as [| a l1 IH].
+  - auto.
+  - inverts Hsubset as Ha Hsubset. specialize (IH Hsubset).
+    (* Take care of the simple case where IH has already found x in l1. *)
+    destruct IH as [IH | IH]. { auto. }
+    apply in_app_or in Ha.
+    destruct Ha as [Ha | [Ha | Ha]]; auto using in_or_app.
+Qed.
+
+Theorem pigeonhole_principle : forall (X : Type) (l1 l2 : list X),
+  Forall (fun x => In x l2) l1 ->
+  length l2 < length l1 ->
+  repeats l1.
+Proof.
+  intros X l1. induction l1 as [| x l1 IH]; introv Hsubset Hlonger.
+  - inverts Hlonger.
+  - (* Proof sketch: if [In x l1], we win. Otherwise, remove x from l2,
+       which lets us preserve [Hlonger] for the induction hypothesis.
+
+       How do we decide if [In x l1], though?
+
+       Answer: [Hsubset] implicitly knows, for each element of [l1], where
+       it occurs in [l2]. Well, at least one occurrence of each. *)
+
+    (* First, we locate at least one occurrence of [x] in [l2]: *)
+    inverts Hsubset as Hx Hsubset.
+
+    (* This is the occurrence we'll be trying to remove for our induction step: *)
+    apply in_split in Hx.
+    destruct Hx as [l2a [l2b El2]]. subst l2.
+
+    (* Iterate over [l1] and see if [Hsubset] ever points at that [x]. If so,
+       [In x l1]. Otherwise we have the precondition of [IH]. *)
+    apply insplit_decide in Hsubset.
+    destruct Hsubset as [Hx | Hsubset]. { auto. }
+    specialize (IH _ Hsubset).
+
+    autorewrite with list in Hlonger, IH. simpl length in Hlonger.
+    apply repeats_cons, IH.
+    lia.
+Qed.
